ThreadBoundedExecution.v -> FinThreads.v

src/basic/FinThreads.v
@@ -4,9 +4,28 @@ From imm Require Import Execution Events.
 Require Import Lia.
 Require Import AuxRel2.
 
+Definition fin_threads G := set_finite (threads_set G).
 
 Definition threads_bound (G: execution) (b: thread_id) :=
   forall e (Ge: acts_set G e), BinPos.Pos.lt (tid e) b.
+
+Lemma fin_threads_bound G (WF: Wf G) (FIN : fin_threads G) :
+  exists b, threads_bound G b.
+Proof using.
+  do 2 red in FIN. desf.
+  unfold threads_bound.
+  enough (exists b, forall t, List.In t findom -> BinPos.Pos.lt t b) as [b HH].
+  { exists b. ins. apply HH. apply FIN. now apply WF. }
+  clear. induction findom.
+  { exists BinPos.xH. ins. }
+  desf.
+  exists (Basic.Ident.add (BinPos.Pos.max a b) BinPos.xH).
+  ins. desf.
+  { lia. }
+  etransitivity.
+  { now apply IHfindom. }
+  lia.
+Qed.
 
 Lemma BinPos_lt_fin b:
   set_finite (fun t => BinPos.Pos.lt t b). 
@@ -27,10 +46,11 @@ Proof using.
   specialize (IHl DUP); desf; eexists (_ :: _); ins; eauto.
 Qed.
 
-Lemma has_finite_antichains_sb (G: execution) b (WF: Wf G) (B: threads_bound G b):
+Lemma has_finite_antichains_sb (G: execution) (WF: Wf G) (B : fin_threads G):
   has_finite_antichains (acts_set G \₁ is_init) (⦗set_compl is_init⦘ ⨾ sb G).
 Proof using.
-  set (nb := BinPos.Pos.to_nat b). 
+  edestruct fin_threads_bound as [b HH]; eauto.
+  set (nb := BinPos.Pos.to_nat b).
   red. exists nb. red. ins.  
   cut (exists a b, a <> b /\ In a l /\ In b l /\ tid a = tid b).
   { intro X; desc.
@@ -39,12 +59,12 @@ Proof using.
     1: exists a, b0. 2: exists b0, a. 
     all: splits; eauto; basic_solver. }
   assert (M: incl (map tid l) (map BinPos.Pos.of_nat (List.seq 0 nb))).
-  { red; ins; rewrite in_map_iff in *; desf.
+  { red. intros n IN. rewrite in_map_iff in *. destruct IN as [x [TT IN]]; subst.
     exists (BinPos.Pos.to_nat (tid x)). split.
     { apply Pnat.Pos2Nat.id. }
     apply in_seq0_iff.
     subst nb. apply Pnat.Pos2Nat.inj_lt.
-    apply B, INCL. auto. }
+    apply HH. now apply INCL. }
   destruct (classic (NoDup (map tid l))).
   { eapply NoDup_incl_length in M; ins.
     rewrite !length_map, length_seq in *. lia. }
@@ -57,8 +77,8 @@ Proof using.
   intro; desf; rewrite nodup_app, nodup_cons in *; desf; eauto with hahn.
 Qed.
 
-Lemma thread_bounds_fsupp_ninit_ct G b r (WF: Wf G)
-      (TB: threads_bound G b)
+Lemma thread_bounds_fsupp_ninit_ct G r (WF: Wf G)
+      (TB : fin_threads G)
       (SB_R: sb G ⊆ r)
       (AC_R: acyclic r)
       (R_NI: domb r (set_compl is_init))
