src/hardware/HardwareFairness.v
@@ -9,7 +9,7 @@ Require Import Execution.
 Require Import Execution_eco.
 Require Import ImmFair.
 Require Import FairExecution.
-Require Import ThreadBoundedExecution.
+Require Import FinThreads.
 Require Import Lia.
 Require Import ClassicalChoice.
 Require Import ChoiceFacts.
@@ -18,47 +18,10 @@ Require Import AuxRel2.
 Require Import AuxDef.
 Require Import Program.Basics.
 Import ListNotations.
+Require Import EnumProperties.
 
 
 Set Implicit Arguments.
-
-Section EnumProperties.
-  Context {A: Type} (r: relation A) (f: nat -> A). 
-
-Lemma enum_exact_steps
-      (STEPS: forall i : nat, r (f i) (f (i + 1))):
-  forall i d, r ^^ d (f i) (f (i + d)). 
-Proof using. 
-  intros. induction d. 
-  { simpl. rewrite PeanoNat.Nat.add_0_r. vauto. }
-  eexists. split; eauto.
-  rewrite NPeano.Nat.add_succ_r, <- NPeano.Nat.add_1_r.
-  apply STEPS. 
-Qed.   
-  
-Lemma enum_steps
-      (STEPS: forall i : nat, r (f i) (f (i + 1))):
-  ⟪STEPS: forall i j (LT: i < j), r^+ (f i) (f j) ⟫. 
-Proof using.
-  red. ins. apply PeanoNat.Nat.le_exists_sub in LT. desc. subst j.
-  apply ctEE. exists p. split; auto.
-  rewrite NPeano.Nat.add_comm, PeanoNat.Nat.add_succ_comm.
-  apply enum_exact_steps. auto. 
-Qed.
-
-Lemma enum_inj
-      (STEPS: forall i, r (f i) (f (i + 1)))
-      (AC: acyclic r):
-  forall x y, f x = f y -> x = y. 
-Proof using. 
-  ins. forward eapply enum_steps as STEPS'; eauto.
-  pose proof (NPeano.Nat.lt_trichotomy x y) as LT.
-  des; auto;
-    destruct (AC (f x)); [rewrite H at 2| rewrite H at 1]; 
-    specialize (STEPS' _ _ LT); auto.
-Qed. 
-
-End EnumProperties. 
 
 Section HardwareFairness.
 
