src/imm/SubExecution.v
@@ -9,7 +9,7 @@ Require Import Events.
 Require Import Execution.
 Require Import FinExecution.
 Require Import FairExecution.
-Require Import ThreadBoundedExecution.
+Require Import FinThreads.
 Require Import Execution_eco.
 Require Import imm_bob imm_s_ppo.
 Require Import imm_s_hb.
