src/lib/EnumProperties.v
@@ -1,0 +1,51 @@
+From hahn Require Import Hahn.
+Require Import AuxRel2.
+Require Import AuxDef. 
+Require Import Basics. 
+Require Import SetSize. 
+Section EnumProperties.
+  Context {A: Type} (r: relation A) (f: nat -> A). 
+
+Lemma enum_exact_steps
+      (STEPS: forall i : nat, r (f i) (f (i + 1))):
+  forall i d, r ^^ d (f i) (f (i + d)). 
+Proof using. 
+  intros. induction d. 
+  { simpl. rewrite PeanoNat.Nat.add_0_r. vauto. }
+  eexists. split; eauto.
+  rewrite NPeano.Nat.add_succ_r, <- NPeano.Nat.add_1_r.
+  apply STEPS. 
+Qed.   
+  
+Lemma enum_steps
+      (STEPS: forall i : nat, r (f i) (f (i + 1))):
+  ⟪STEPS: forall i j (LT: i < j), r^+ (f i) (f j) ⟫. 
+Proof using.
+  red. ins. apply PeanoNat.Nat.le_exists_sub in LT. desc. subst j.
+  apply ctEE. exists p. split; auto.
+  rewrite NPeano.Nat.add_comm, PeanoNat.Nat.add_succ_comm.
+  apply enum_exact_steps. auto. 
+Qed.
+
+Lemma enum_inj
+      (STEPS: forall i, r (f i) (f (i + 1)))
+      (AC: acyclic r):
+  forall x y, f x = f y -> x = y. 
+Proof using. 
+  ins. forward eapply enum_steps as STEPS'; eauto.
+  pose proof (NPeano.Nat.lt_trichotomy x y) as LT.
+  des; auto;
+    destruct (AC (f x)); [rewrite H at 2| rewrite H at 1]; 
+    specialize (STEPS' _ _ LT); auto.
+Qed. 
+
+Lemma enumerates_set_bunion (steps: nat -> A) (S: A -> Prop)
+  (ENUM: enumerates steps S):
+  S ≡₁ ⋃₁ i ∈ flip NOmega.lt_nat_l (set_size S), eq (steps i).
+Proof using. 
+  apply enumeratesE' in ENUM. desc.
+  split; unfolder; ins; desc; subst. 
+  by apply INSET.
+Qed.
+
+End EnumProperties. 
